feat: add lemmas of translation properties
also cleaned up and documented project

theories/Printer.v
@@ -1,24 +1,20 @@
 From Coq Require Import String BinInt List.
 
-(* printing functionality *)
+(* printer for dumping pretty-printed PIR terms to check with the Plutus CLI tool *)
 From SimpleIO Require Import SimpleIO.
+From QuickChick Require Import Show.
 
-From VTL Require Import Env PIR Pretty Translation.
+From VTL Require Import PIR Pretty Translation.
 
 Import PlutusNotations ListNotations.
 Local Open Scope string_scope.
 Local Open Scope Z_scope.
 
 Definition identity_ast : term :=
-  <{ λ "x" :: ℤ, {Var "x"} }>
-.
+  <{ λ "x" :: ℤ, {Var "x"} }>.
 
 Definition plus_ast : term :=
   <{ (λ "x" :: ℤ, λ "y" :: ℤ, {Var "x"} + {Var "y"}) ⋅ CInt 1 }>.
-
-(* Definition let_ast : term :=
- (Let NonRec [(TermBind Strict (VarDecl "x" ℤ) (Error ℤ))] 
-    <{ CInt 10 + {Var "x"} + CInt 5 }>). *)
 
 Import IO.Notations.
 
@@ -27,12 +23,13 @@ RunIO IOMode Forward.
 (* Automatically assign the right integer types (hopefully) *)
 RunIO Smart On.
 
+(* We test the pipeline starting from the λ□ identity function *)
 Definition test_pir_ast := (translate_unsafe nil identity_EAst ann_id).
 Eval cbv in (print_as_program test_pir_ast).
 Definition main : IO unit :=
   chan <- open_out "./output/test.pir" ;;
   output_string chan (print_as_program test_pir_ast) ;;
-  close_out chan
-.
+  close_out chan.
 
+(* Getting errors: PrimFloat.float PrimInt63.int have to be realized *)
 (* RunIO main. *)
