output/test.pir
@@ -1,1 +1,1 @@
-(program 1.1.0 (lam x (con integer) x))
+(program 1.1.0 (lam y (con integer) y))
